common/Memory.v
@@ -44,7 +44,7 @@ Require Export Memtype.
 (* To avoid useless definitions of inductors in extracted code. *)
 Local Unset Elimination Schemes.
 Local Unset Case Analysis Schemes.
-
+(*
 Module NMap.
   Definition elt := block.
   Definition elt_eq := eq_block.
@@ -208,10 +208,11 @@ Proof.
 Qed.
 
 End Sup.
-
+*)
 Module Mem <: MEM.
-Include Sup.
-Local Notation "a # b" := (NMap.get _ b a) (at level 1).
+  (* Include Sup. *)
+  
+Local Notation "a # b" := (PMap.get b a) (at level 1).
 Local Notation "a ## b" := (ZMap.get b a) (at level 1).
 
 Definition perm_order' (po: option permission) (p: permission) :=
@@ -231,15 +232,15 @@ Definition memperm : Type := perm_kind -> option permission.
 
 
 Record mem' : Type := mkmem {
-  mem_contents: NMap.t (ZMap.t memval);  (**r [block -> offset -> memval] *)
-  mem_access: NMap.t (ZMap.t memperm);
+  mem_contents: PMap.t (ZMap.t memval);  (**r [block -> offset -> memval] *)
+  mem_access: PMap.t (ZMap.t memperm);
                                          (**r [block -> offset -> kind -> option permission] *)
-  support: sup;
+  nextblock: block;
 
   access_max:
     forall b ofs, perm_order'' (mem_access#b##ofs Max) (mem_access#b ## ofs Cur);
   nextblock_noaccess:
-    forall b ofs k, ~(sup_In b support) -> mem_access#b##ofs k = None;
+    forall b ofs k, ~(Plt b nextblock) -> mem_access#b##ofs k = None;
   contents_default:
     forall b, fst (mem_contents#b) = Undef;
   access_default:
@@ -248,12 +249,11 @@ Record mem' : Type := mkmem {
 
 Definition mem := mem'.
 
-Definition nextblock (m:mem) := fresh_block (support m).
 
 Lemma mkmem_ext:
- forall cont1 cont2 acc1 acc2 sup1 sup2 a1 a2 b1 b2 c1 c2 d1 d2,
-  cont1=cont2 -> acc1=acc2 -> sup1=sup2 ->
-  mkmem cont1 acc1 sup1 a1 b1 c1 d1= mkmem cont2 acc2 sup2 a2 b2 c2 d2.
+ forall cont1 cont2 acc1 acc2 next1 NEXT2 a1 a2 b1 b2 c1 c2 d1 d2,
+  cont1=cont2 -> acc1=acc2 -> next1=NEXT2 ->
+  mkmem cont1 acc1 next1 a1 b1 c1 d1= mkmem cont2 acc2 NEXT2 a2 b2 c2 d2.
 Proof.
   intros. subst. f_equal; apply proof_irr.
 Qed.
@@ -263,7 +263,7 @@ Qed.
 (** A block address is valid if it was previously allocated. It remains valid
   even after being freed. *)
 
-Definition valid_block (m: mem) (b: block) := sup_In b (support m).
+Definition valid_block (m: mem) (b: block) := Plt b (nextblock m).
 
 Theorem valid_not_valid_diff:
   forall m b b', valid_block m b -> ~(valid_block m b') -> b <> b'.
@@ -319,7 +319,7 @@ Theorem perm_valid_block:
   forall m b ofs k p, perm m b ofs k p -> valid_block m b.
 Proof.
   unfold perm; intros.
-  destruct (sup_dec b m.(support)).
+  destruct (plt b m.(nextblock)).
   auto.
   assert (m.(mem_access)#b## ofs k = None).
   eapply nextblock_noaccess; eauto.
@@ -517,15 +517,11 @@ Qed.
 (** The initial store *)
 
 Program Definition empty: mem :=
-  mkmem (NMap.init _ (ZMap.init Undef))
-        (NMap.init _ (ZMap.init (fun k => None)))
-        sup_empty  _ _ _ _.
+  mkmem (PMap.init (ZMap.init Undef))
+        (PMap.init (ZMap.init (fun k => None)))
+        1%positive _ _ _ _.
 
-(** Allocation of a fresh block with the given bounds.  Return an updated
-  memory state and the address of the fresh block, which initially contains
-  undefined cells.  Note that allocation never fails: we model an
-  infinite memory. *)
-Lemma mem_incr_1: forall m, sup_In (nextblock m) (sup_incr (m.(support))).
+(* Lemma mem_incr_1: forall m, sup_In (nextblock m) (sup_incr (m.(support))).
 Proof.
   intros. unfold nextblock. unfold sup_incr. apply sup_incr_in1.
 Qed.
@@ -534,7 +530,7 @@ Lemma mem_incr_2: forall m b, sup_In b (m.(support)) -> sup_In b (sup_incr (m.(s
 Proof.
   intros. unfold sup_incr. apply sup_incr_in2. auto.
 Qed.
-
+*)
 (** Writing N adjacent bytes in a block memperm. *)
 
 Definition interval_length (lo: Z) (hi: Z) : nat :=
@@ -640,34 +636,39 @@ Proof.
   eapply setpermN'_default; eauto.
 Qed.
 
+ (** Allocation of a fresh block with the given bounds.  Return an updated
+  memory state and the address of the fresh block, which initially contains
+  undefined cells.  Note that allocation never fails: we model an
+  infinite memory. *)
+
 Program Definition alloc (m: mem) (lo hi: Z) :=
-  (mkmem (NMap.set _ (nextblock m)
+  (mkmem (PMap.set (nextblock m)
                    (ZMap.init Undef)
                    m.(mem_contents))
-         (NMap.set _ (nextblock m)
+         (PMap.set (nextblock m)
                    (setpermN lo hi (Some Freeable) (ZMap.init (fun k => None)))
                    m.(mem_access))
-         (sup_incr (m.(support)))
+         (Pos.succ (m.(nextblock)))
          _ _ _ _,
    (nextblock m)).
 Next Obligation.
-  repeat rewrite NMap.gsspec. destruct (NMap.elt_eq b (nextblock m)).
+  repeat rewrite PMap.gsspec. destruct (peq b (nextblock m)).
   subst b. rewrite setpermN_inv.
   destruct (zle lo ofs && zlt ofs hi). constructor.
   simpl. auto.
   apply access_max.
 Qed.
 Next Obligation.
-  rewrite NMap.gsspec. destruct (NMap.elt_eq b (nextblock m)).
-  subst b. elim H. apply mem_incr_1.
+  rewrite PMap.gsspec. destruct (peq b (nextblock m)).
+  subst b. elim H. apply Plt_succ.
   apply nextblock_noaccess. red; intros; elim H.
-  apply mem_incr_2. auto.
+  apply Plt_trans_succ; auto.
 Qed.
 Next Obligation.
-  rewrite NMap.gsspec. destruct (NMap.elt_eq b (nextblock m)). auto. apply contents_default.
+  rewrite PMap.gsspec. destruct (peq b (nextblock m)). auto. apply contents_default.
 Qed.
 Next Obligation.
-  rewrite NMap.gsspec. destruct (NMap.elt_eq b (nextblock m)). auto.
+  rewrite PMap.gsspec. destruct (peq b (nextblock m)). auto.
   rewrite setpermN_default. auto. apply access_default.
 Qed.
 
@@ -678,19 +679,19 @@ Qed.
 
 Program Definition unchecked_free (m: mem) (b: block) (lo hi: Z): mem :=
   mkmem m.(mem_contents)
-        (NMap.set _ b
+        (PMap.set b
                 (setpermN lo hi None (m.(mem_access)#b))
                 m.(mem_access))
-        m.(support) _ _ _ _.
+        m.(nextblock) _ _ _ _.
 Next Obligation.
-  repeat rewrite NMap.gsspec. destruct (NMap.elt_eq b0 b).
+  repeat rewrite PMap.gsspec. destruct (peq b0 b).
   subst.
   rewrite setpermN_inv.
   destruct (zle lo ofs && zlt ofs hi). constructor.
   apply access_max.  apply access_max.
 Qed.
 Next Obligation.
-  repeat rewrite NMap.gsspec. destruct (NMap.elt_eq b0 b). subst.
+  repeat rewrite PMap.gsspec. destruct (peq b0 b). subst.
   destruct (Z_le_dec lo ofs); destruct (Z_lt_dec ofs hi).
   rewrite setpermN_inside. constructor. lia.
   rewrite setpermN_outside. apply nextblock_noaccess; auto. lia.
@@ -702,7 +703,7 @@ Next Obligation.
   apply contents_default.
 Qed.
 Next Obligation.
-  rewrite NMap.gsspec. destruct (NMap.elt_eq b0 b). subst.
+  rewrite PMap.gsspec. destruct (peq b0 b). subst.
   rewrite setpermN_default.
   apply access_default.
   apply access_default.
@@ -844,18 +845,18 @@ Qed.
 
 Program Definition store (chunk: memory_chunk) (m: mem) (b: block) (ofs: Z) (v: val): option mem :=
   if valid_access_dec m chunk b ofs Writable then
-    Some (mkmem (NMap.set _ b
+    Some (mkmem (PMap.set b
                           (setN (encode_val chunk v) ofs (m.(mem_contents)#b))
                           m.(mem_contents))
                 m.(mem_access)
-                m.(support)
+                m.(nextblock)
                 _ _ _ _)
   else
     None.
 Next Obligation. apply access_max. Qed.
 Next Obligation. apply nextblock_noaccess; auto. Qed.
 Next Obligation.
-  rewrite NMap.gsspec. destruct (NMap.elt_eq b0 b).
+  rewrite PMap.gsspec. destruct (peq b0 b).
   rewrite setN_default. apply contents_default.
   apply contents_default.
 Qed.
@@ -870,19 +871,6 @@ Definition storev (chunk: memory_chunk) (m: mem) (addr v: val) : option mem :=
   | _ => None
   end.
 
-Theorem support_storev: forall chunk m addr v m',
-    storev chunk m addr v = Some m' -> support m = support m'.
-Proof.
-  intros.
-  unfold storev in H.
-  unfold store in H.
-  destruct addr; try congruence.
-  destruct (valid_access_dec m chunk b (Ptrofs.unsigned i) Writable).
-  inv H.
-  auto.
-  congruence.
-Qed.
-
 (** [storebytes m b ofs bytes] stores the given list of bytes [bytes]
   starting at location [(b, ofs)].  Returns updated memory state
   or [None] if the accessed locations are not writable. *)
@@ -890,16 +878,16 @@ Qed.
 Program Definition storebytes (m: mem) (b: block) (ofs: Z) (bytes: list memval) : option mem :=
   if range_perm_dec m b ofs (ofs + Z.of_nat (length bytes)) Cur Writable then
     Some (mkmem
-             (NMap.set _ b (setN bytes ofs (m.(mem_contents)#b)) m.(mem_contents))
+             (PMap.set b (setN bytes ofs (m.(mem_contents)#b)) m.(mem_contents))
              m.(mem_access)
-             m.(support)
+             m.(nextblock)
              _ _ _ _)
   else
     None.
 Next Obligation. apply access_max. Qed.
 Next Obligation. apply nextblock_noaccess; auto. Qed.
 Next Obligation.
-  rewrite NMap.gsspec. destruct (NMap.elt_eq b0 b).
+  rewrite PMap.gsspec. destruct (peq b0 b).
   rewrite setN_default. apply contents_default.
   apply contents_default.
 Qed.
@@ -913,19 +901,19 @@ Next Obligation. apply access_default. Qed.
 Program Definition drop_perm (m: mem) (b: block) (lo hi: Z) (p: permission): option mem :=
   if range_perm_dec m b lo hi Cur Freeable then
     Some (mkmem m.(mem_contents)
-                (NMap.set _ b
+                (PMap.set b
                         (setpermN lo hi (Some p) (mem_access m) # b)
                         m.(mem_access))
-                m.(support) _ _ _ _)
+                m.(nextblock) _ _ _ _)
   else None.
 Next Obligation.
-  repeat rewrite NMap.gsspec. destruct (NMap.elt_eq b0 b). subst b0.
+  repeat rewrite PMap.gsspec. destruct (peq b0 b). subst b0.
   rewrite setpermN_inv. destruct (zle lo ofs && zlt ofs hi).
   constructor. apply access_max. apply access_max.
 Qed.
 Next Obligation.
   specialize (nextblock_noaccess m b0 ofs k H0). intros.
-  rewrite NMap.gsspec. destruct (NMap.elt_eq b0 b). subst b0.
+  rewrite PMap.gsspec. destruct (peq b0 b). subst b0.
   rewrite setpermN_inv.
   destruct (zle lo ofs); destruct (zlt ofs hi); simpl.
   assert (perm m b ofs k Freeable). apply perm_cur. apply H; auto.
@@ -936,7 +924,7 @@ Next Obligation.
   apply contents_default.
 Qed.
 Next Obligation.
-  rewrite NMap.gsspec. destruct (NMap.elt_eq b0 b). subst b0.
+  rewrite PMap.gsspec. destruct (peq b0 b). subst b0.
   rewrite setpermN_default.
   apply access_default. apply access_default.
 Qed.
@@ -944,7 +932,7 @@ Qed.
 (** * Properties of the memory operations *)
 
 (** Properties of the empty store. *)
-Theorem support_empty : support empty = sup_empty.
+Theorem nextblock_empty : nextblock empty = 1%positive.
 Proof.
   reflexivity.
 Qed.
@@ -1304,7 +1292,7 @@ Proof.
 Qed.
 
 Lemma store_mem_contents:
-  mem_contents m2 = NMap.set _ b (setN (encode_val chunk v) ofs m1.(mem_contents)#b) m1.(mem_contents).
+  mem_contents m2 = PMap.set b (setN (encode_val chunk v) ofs m1.(mem_contents)#b) m1.(mem_contents).
 Proof.
   unfold store in STORE. destruct (valid_access_dec m1 chunk b ofs Writable); inv STORE.
   auto.
@@ -1333,24 +1321,16 @@ Proof.
   auto.
 Qed.
 
-Theorem support_store:
-  support m2 = support m1.
-Proof.
-  intros.
-  unfold store in STORE. destruct ( valid_access_dec m1 chunk b ofs Writable); inv STORE.
-  auto.
-Qed.
-
 Theorem store_valid_block_1:
   forall b', valid_block m1 b' -> valid_block m2 b'.
 Proof.
-  unfold valid_block; intros. rewrite support_store; auto.
+  unfold valid_block; intros. rewrite nextblock_store; auto.
 Qed.
 
 Theorem store_valid_block_2:
   forall b', valid_block m2 b' -> valid_block m1 b'.
 Proof.
-  unfold valid_block; intros. rewrite support_store in H; auto.
+  unfold valid_block; intros. rewrite nextblock_store in H; auto.
 Qed.
 
 Local Hint Resolve store_valid_block_1 store_valid_block_2: mem.
@@ -1392,7 +1372,7 @@ Proof.
   exists v'; split; auto.
   exploit load_result; eauto. intros B.
   rewrite B. rewrite store_mem_contents; simpl.
-  setoid_rewrite NMap.gss.
+  setoid_rewrite PMap.gss.
   replace (size_chunk_nat chunk') with (length (encode_val chunk v)).
   rewrite getN_setN_same. apply decode_encode_val_general.
   rewrite encode_val_length. repeat rewrite size_chunk_conv in H.
@@ -1427,7 +1407,7 @@ Proof.
   destruct (valid_access_dec m1 chunk' b' ofs' Readable).
   rewrite pred_dec_true.
   decEq. decEq. rewrite store_mem_contents; simpl.
-  rewrite NMap.gsspec. destruct (NMap.elt_eq b' b). subst b'.
+  rewrite PMap.gsspec. destruct (peq b' b). subst b'.
   apply getN_setN_outside. rewrite encode_val_length. repeat rewrite <- size_chunk_conv.
   intuition.
   auto.
@@ -1442,7 +1422,7 @@ Proof.
   intros.
   assert (valid_access m2 chunk b ofs Readable) by eauto with mem.
   unfold loadbytes. rewrite pred_dec_true. rewrite store_mem_contents; simpl.
-  setoid_rewrite NMap.gss.
+  setoid_rewrite PMap.gss.
   replace (Z.to_nat (size_chunk chunk)) with (length (encode_val chunk v)).
   rewrite getN_setN_same. auto.
   rewrite encode_val_length. auto.
@@ -1461,7 +1441,7 @@ Proof.
   destruct (range_perm_dec m1 b' ofs' (ofs' + n) Cur Readable).
   rewrite pred_dec_true.
   decEq. rewrite store_mem_contents; simpl.
-  rewrite NMap.gsspec. destruct (NMap.elt_eq b' b). subst b'.
+  rewrite PMap.gsspec. destruct (peq b' b). subst b'.
   destruct H. congruence.
   destruct (zle n 0) as [z | n0].
   rewrite (Z_to_nat_neg _ z). auto.
@@ -1521,7 +1501,7 @@ Lemma load_store_overlap:
 Proof.
   intros.
   exploit load_result; eauto. erewrite store_mem_contents by eauto; simpl.
-  setoid_rewrite NMap.gss.
+  setoid_rewrite PMap.gss.
   set (c := (mem_contents m1)#b). intros V'.
   destruct (size_chunk_nat_pos chunk) as [sz SIZE].
   destruct (size_chunk_nat_pos chunk') as [sz' SIZE'].
@@ -1583,7 +1563,7 @@ Theorem load_pointer_store:
   \/ (b' <> b \/ ofs' + size_chunk chunk' <= ofs \/ ofs + size_chunk chunk <= ofs').
 Proof.
   intros.
-  destruct (NMap.elt_eq b' b); auto. subst b'.
+  destruct (peq b' b); auto. subst b'.
   destruct (zle (ofs' + size_chunk chunk') ofs); auto.
   destruct (zle (ofs + size_chunk chunk) ofs'); auto.
   exploit load_store_overlap; eauto.
@@ -1772,14 +1752,6 @@ Variable bytes: list memval.
 Variable m2: mem.
 Hypothesis STORE: storebytes m1 b ofs bytes = Some m2.
 
-Lemma storebytes_empty : bytes = nil -> m1 = m2.
-  intro. subst. inv STORE. unfold storebytes in H0.
-  destruct range_perm_dec; try congruence.
-  inv H0. destruct m1.
-  apply mkmem_ext; eauto. cbn.
-  apply NMap.set3.
-Qed.
-
 Lemma storebytes_access: mem_access m2 = mem_access m1.
 Proof.
   unfold storebytes in STORE.
@@ -1789,7 +1761,7 @@ Proof.
 Qed.
 
 Lemma storebytes_mem_contents:
-   mem_contents m2 = NMap.set _ b (setN bytes ofs m1.(mem_contents)#b) m1.(mem_contents).
+   mem_contents m2 = PMap.set b (setN bytes ofs m1.(mem_contents)#b) m1.(mem_contents).
 Proof.
   unfold storebytes in STORE.
   destruct (range_perm_dec m1 b ofs (ofs + Z.of_nat (length bytes)) Cur Writable);
@@ -1837,26 +1809,16 @@ Proof.
   auto.
 Qed.
 
-Theorem support_storebytes:
-  support m2 = support m1.
-Proof.
-  intros.
-  unfold storebytes in STORE.
-  destruct (range_perm_dec m1 b ofs (ofs + Z.of_nat (length bytes)) Cur Writable);
-  inv STORE.
-  auto.
-Qed.
-
 Theorem storebytes_valid_block_1:
   forall b', valid_block m1 b' -> valid_block m2 b'.
 Proof.
-  unfold valid_block; intros. rewrite support_storebytes; auto.
+  unfold valid_block; intros. rewrite nextblock_storebytes; auto.
 Qed.
 
 Theorem storebytes_valid_block_2:
   forall b', valid_block m2 b' -> valid_block m1 b'.
 Proof.
-  unfold valid_block; intros. rewrite support_storebytes in H; auto.
+  unfold valid_block; intros. rewrite nextblock_storebytes in H; auto.
 Qed.
 
 Local Hint Resolve storebytes_valid_block_1 storebytes_valid_block_2: mem.
@@ -1878,7 +1840,7 @@ Proof.
   destruct (range_perm_dec m1 b ofs (ofs + Z.of_nat (length bytes)) Cur Writable);
   try discriminate.
   rewrite pred_dec_true.
-  decEq. inv STORE2; simpl. setoid_rewrite NMap.gss. rewrite Nat2Z.id.
+  decEq. inv STORE2; simpl. setoid_rewrite PMap.gss. rewrite Nat2Z.id.
   apply getN_setN_same.
   red; eauto with mem.
 Qed.
@@ -1893,7 +1855,7 @@ Proof.
   destruct (range_perm_dec m1 b' ofs' (ofs' + len) Cur Readable).
   rewrite pred_dec_true.
   rewrite storebytes_mem_contents. decEq.
-  rewrite NMap.gsspec. destruct (NMap.elt_eq b' b). subst b'.
+  rewrite PMap.gsspec. destruct (peq b' b). subst b'.
   apply getN_setN_disjoint. rewrite Z2Nat.id by lia. intuition congruence.
   auto.
   red; auto with mem.
@@ -1924,7 +1886,7 @@ Proof.
   destruct (valid_access_dec m1 chunk b' ofs' Readable).
   rewrite pred_dec_true.
   rewrite storebytes_mem_contents. decEq.
-  rewrite NMap.gsspec. destruct (NMap.elt_eq b' b). subst b'.
+  rewrite PMap.gsspec. destruct (peq b' b). subst b'.
   rewrite getN_setN_outside. auto. rewrite <- size_chunk_conv. intuition congruence.
   auto.
   destruct v; split; auto. red; auto with mem.
@@ -1955,7 +1917,7 @@ Proof.
   destruct (range_perm_dec m1 b (ofs + Z.of_nat(length bytes1)) (ofs + Z.of_nat(length bytes1) + Z.of_nat(length bytes2)) Cur Writable); try congruence.
   destruct (range_perm_dec m b ofs (ofs + Z.of_nat (length (bytes1 ++ bytes2))) Cur Writable).
   inv ST1; inv ST2; simpl. decEq. apply mkmem_ext; auto.
-  setoid_rewrite NMap.gss.  rewrite setN_concat. symmetry. apply NMap.set2.
+  setoid_rewrite PMap.gss.  rewrite setN_concat. symmetry. apply PMap.set2.
   elim n.
   rewrite app_length. rewrite Nat2Z.inj_add. red; intros.
   destruct (zlt ofs0 (ofs + Z.of_nat(length bytes1))).
@@ -2031,16 +1993,11 @@ Variable b: block.
 Hypothesis ALLOC: alloc m1 lo hi = (m2, b).
 
 Theorem nextblock_alloc:
-  nextblock m2 = fresh_block (sup_incr(support m1)).
+  nextblock m2 = Pos.succ (nextblock m1).
 Proof.
   injection ALLOC; intros. rewrite <- H0; auto.
 Qed.
 
-Theorem support_alloc:
-  support m2 = sup_incr(support m1).
-Proof.
-  injection ALLOC; intros. rewrite <- H0; auto.
-Qed.
 Theorem alloc_result:
   b = nextblock m1.
 Proof.
@@ -2050,20 +2007,20 @@ Qed.
 Theorem valid_block_alloc:
   forall b', valid_block m1 b' -> valid_block m2 b'.
 Proof.
-  unfold valid_block; intros. rewrite support_alloc.
-  apply mem_incr_2. auto.
+  unfold valid_block; intros. rewrite nextblock_alloc.
+  apply Plt_trans_succ. auto.
 Qed.
 
 Theorem fresh_block_alloc:
   ~(valid_block m1 b).
 Proof.
-  unfold valid_block. rewrite alloc_result. apply freshness.
+  unfold valid_block. rewrite alloc_result. apply Plt_strict.
 Qed.
 
 Theorem valid_new_block:
   valid_block m2 b.
 Proof.
-  unfold valid_block. rewrite alloc_result. rewrite support_alloc. apply mem_incr_1.
+  unfold valid_block. rewrite alloc_result. rewrite nextblock_alloc. apply Plt_succ.
 Qed.
 
 Local Hint Resolve valid_block_alloc fresh_block_alloc valid_new_block: mem.
@@ -2072,23 +2029,23 @@ Theorem valid_block_alloc_inv:
   forall b', valid_block m2 b' -> b' = b \/ valid_block m1 b'.
 Proof.
   unfold valid_block; intros.
-  rewrite support_alloc in H. rewrite alloc_result.
-  apply sup_incr_in. auto.
+  rewrite nextblock_alloc in H. rewrite alloc_result.
+  exploit Plt_succ_inv; eauto. tauto.
 Qed.
 
 Theorem perm_alloc_1:
   forall b' ofs k p, perm m1 b' ofs k p -> perm m2 b' ofs k p.
 Proof.
   unfold perm; intros. injection ALLOC; intros. rewrite <- H1; simpl.
-  subst b. rewrite NMap.gsspec. destruct (NMap.elt_eq b' (nextblock m1)); auto.
-  rewrite nextblock_noaccess in H. contradiction. subst b'. apply freshness.
+  subst b. rewrite PMap.gsspec. destruct (peq b' (nextblock m1)); auto.
+  rewrite nextblock_noaccess in H. contradiction. subst b'. apply Plt_strict.
 Qed.
 
 Theorem perm_alloc_2:
   forall ofs k, lo <= ofs < hi -> perm m2 b ofs k Freeable.
 Proof.
   unfold perm; intros. injection ALLOC; intros. rewrite <- H1; simpl.
-  subst b. unfold NMap.get. rewrite NMap.gss.
+  subst b. rewrite PMap.gss.
   rewrite setpermN_inside. simpl. auto with mem. lia.
 Qed.
 
@@ -2098,7 +2055,7 @@ Theorem perm_alloc_inv:
   if eq_block b' b then lo <= ofs < hi else perm m1 b' ofs k p.
 Proof.
   intros until p; unfold perm. inv ALLOC. simpl.
-  rewrite NMap.gsspec.  destruct (NMap.elt_eq b' (nextblock m1)); intros.
+  rewrite PMap.gsspec.  destruct (peq b' (nextblock m1)); intros.
   assert (zle lo ofs && zlt ofs hi = true).
     rewrite setpermN_inv in H.
     destruct(zle lo ofs && zlt ofs hi). reflexivity. contradiction.
@@ -2177,7 +2134,7 @@ Proof.
   subst b'. elimtype False. eauto with mem.
   rewrite pred_dec_true; auto.
   injection ALLOC; intros. rewrite <- H2; simpl.
-  setoid_rewrite NMap.gso. auto. rewrite H1. apply not_eq_sym; eauto with mem.
+  setoid_rewrite PMap.gso. auto. rewrite H1. apply not_eq_sym; eauto with mem.
   rewrite pred_dec_false. auto.
   eauto with mem.
 Qed.
@@ -2197,7 +2154,7 @@ Theorem load_alloc_same:
 Proof.
   intros. exploit load_result; eauto. intro. rewrite H0.
   injection ALLOC; intros. rewrite <- H2; simpl. rewrite <- H1.
-  setoid_rewrite NMap.gss. destruct (size_chunk_nat_pos chunk) as [n E]. rewrite E. simpl.
+  setoid_rewrite PMap.gss. destruct (size_chunk_nat_pos chunk) as [n E]. rewrite E. simpl.
   rewrite ZMap.gi. apply decode_val_undef.
 Qed.
 
@@ -2222,7 +2179,7 @@ Proof.
   destruct (range_perm_dec m1 b' ofs (ofs + n) Cur Readable).
   rewrite pred_dec_true.
   injection ALLOC; intros A B. rewrite <- B; simpl.
-  setoid_rewrite NMap.gso. auto. rewrite A. eauto with mem.
+  setoid_rewrite PMap.gso. auto. rewrite A. eauto with mem.
   red; intros. eapply perm_alloc_1; eauto.
   rewrite pred_dec_false; auto.
   red; intros; elim n0. red; intros. eapply perm_alloc_4; eauto. eauto with mem.
@@ -2235,7 +2192,7 @@ Theorem loadbytes_alloc_same:
 Proof.
   unfold loadbytes; intros. destruct (range_perm_dec m2 b ofs (ofs + n) Cur Readable); inv H.
   revert H0.
-  injection ALLOC; intros A B. rewrite <- A; rewrite <- B; simpl. setoid_rewrite NMap.gss.
+  injection ALLOC; intros A B. rewrite <- A; rewrite <- B; simpl. setoid_rewrite PMap.gss.
   generalize (Z.to_nat n) ofs. induction n0; simpl; intros.
   contradiction.
   rewrite ZMap.gi in H. destruct H; eauto.
@@ -2284,13 +2241,6 @@ Proof.
   rewrite free_result; reflexivity.
 Qed.
 
-Theorem support_free:
-  support m2 = support m1.
-Proof.
-  rewrite free_result; reflexivity.
-Qed.
-
-
 Theorem valid_block_free_1:
   forall b, valid_block m1 b -> valid_block m2 b.
 Proof.
@@ -2312,7 +2262,7 @@ Theorem perm_free_1:
   perm m2 b ofs k p.
 Proof.
   intros. rewrite free_result. unfold perm, unchecked_free; simpl.
-  rewrite NMap.gsspec. destruct (NMap.elt_eq b bf). subst b.
+  rewrite PMap.gsspec. destruct (peq b bf). subst b.
   rewrite setpermN_inv.
   destruct (zle lo ofs); simpl.
   destruct (zlt ofs hi); simpl.
@@ -2325,7 +2275,7 @@ Theorem perm_free_2:
   forall ofs k p, lo <= ofs < hi -> ~ perm m2 bf ofs k p.
 Proof.
   intros. rewrite free_result. unfold perm, unchecked_free; simpl.
-  unfold NMap.get. rewrite NMap.gss.
+  rewrite PMap.gss.
   rewrite setpermN_inv. unfold proj_sumbool.
   rewrite zle_true. rewrite zlt_true.
   simpl. tauto. lia. lia.
@@ -2336,7 +2286,7 @@ Theorem perm_free_3:
   perm m2 b ofs k p -> perm m1 b ofs k p.
 Proof.
   intros until p. rewrite free_result. unfold perm, unchecked_free; simpl.
-  rewrite NMap.gsspec. destruct (NMap.elt_eq b bf). subst b.
+  rewrite PMap.gsspec. destruct (peq b bf). subst b.
   rewrite setpermN_inv.
   destruct (zle lo ofs); simpl.
   destruct (zlt ofs hi); simpl. tauto.
@@ -2349,7 +2299,7 @@ Theorem perm_free_4:
 Proof.
   intros until p.
   rewrite free_result. unfold perm, unchecked_free; simpl.
-  rewrite NMap.gsspec. destruct (NMap.elt_eq b bf). subst b.
+  rewrite PMap.gsspec. destruct (peq b bf). subst b.
   - 
   rewrite setpermN_inv.
   destruct (zle lo ofs); simpl.
@@ -2364,7 +2314,7 @@ Theorem perm_free_inv:
   (b = bf /\ lo <= ofs < hi) \/ perm m2 b ofs k p.
 Proof.
   intros. rewrite free_result. unfold perm, unchecked_free; simpl.
-  rewrite NMap.gsspec. destruct (NMap.elt_eq b bf); auto. subst b.
+  rewrite PMap.gsspec. destruct (peq b bf); auto. subst b.
   rewrite setpermN_inv.
   destruct (zle lo ofs); simpl; auto.
   destruct (zlt ofs hi); simpl; auto.
@@ -2403,7 +2353,7 @@ Proof.
   intros. destruct H. split; auto.
   red; intros. generalize (H ofs0 H1).
   rewrite free_result. unfold perm, unchecked_free; simpl.
-  rewrite NMap.gsspec. destruct (NMap.elt_eq b bf). subst b.
+  rewrite PMap.gsspec. destruct (peq b bf). subst b.
   rewrite setpermN_inv.
   destruct (zle lo ofs0); simpl.
   destruct (zlt ofs0 hi); simpl.
@@ -2508,22 +2458,16 @@ Proof.
   unfold drop_perm in DROP. destruct (range_perm_dec m b lo hi Cur Freeable); inv DROP; auto.
 Qed.
 
-Theorem support_drop:
-  support m' = support m.
-Proof.
-  unfold drop_perm in DROP. destruct (range_perm_dec m b lo hi Cur Freeable); inv DROP; auto.
-Qed.
-
 Theorem drop_perm_valid_block_1:
   forall b', valid_block m b' -> valid_block m' b'.
 Proof.
-  unfold valid_block; rewrite support_drop; auto.
+  unfold valid_block; rewrite nextblock_drop; auto.
 Qed.
 
 Theorem drop_perm_valid_block_2:
   forall b', valid_block m' b' -> valid_block m b'.
 Proof.
-  unfold valid_block; rewrite support_drop; auto.
+  unfold valid_block; rewrite nextblock_drop; auto.
 Qed.
 
 Theorem perm_drop_1:
@@ -2531,7 +2475,7 @@ Theorem perm_drop_1:
 Proof.
   intros.
   unfold drop_perm in DROP. destruct (range_perm_dec m b lo hi Cur Freeable); inv DROP.
-  unfold perm. simpl. unfold NMap.get. rewrite NMap.gss.
+  unfold perm. simpl. rewrite PMap.gss.
   rewrite setpermN_inv. unfold proj_sumbool.
   rewrite zle_true. rewrite zlt_true. simpl. constructor.
   lia. lia.
@@ -2542,7 +2486,7 @@ Theorem perm_drop_2:
 Proof.
   intros.
   unfold drop_perm in DROP. destruct (range_perm_dec m b lo hi Cur Freeable); inv DROP.
-  revert H0. unfold perm; simpl. unfold NMap.get. rewrite NMap.gss.
+  revert H0. unfold perm; simpl. rewrite PMap.gss.
   rewrite setpermN_inv. unfold proj_sumbool.
   rewrite zle_true. rewrite zlt_true. simpl. auto.
   lia. lia.
@@ -2553,7 +2497,7 @@ Theorem perm_drop_3:
 Proof.
   intros.
   unfold drop_perm in DROP. destruct (range_perm_dec m b lo hi Cur Freeable); inv DROP.
-  unfold perm; simpl. rewrite NMap.gsspec. destruct (NMap.elt_eq b' b). subst b'.
+  unfold perm; simpl. rewrite PMap.gsspec. destruct (peq b' b). subst b'.
   rewrite setpermN_inv.
   unfold proj_sumbool. destruct (zle lo ofs). destruct (zlt ofs hi).
   byContradiction. intuition lia.
@@ -2565,7 +2509,7 @@ Theorem perm_drop_4:
 Proof.
   intros.
   unfold drop_perm in DROP. destruct (range_perm_dec m b lo hi Cur Freeable); inv DROP.
-  revert H. unfold perm; simpl. rewrite NMap.gsspec. destruct (NMap.elt_eq b' b).
+  revert H. unfold perm; simpl. rewrite PMap.gsspec. destruct (peq b' b).
   subst b'.  rewrite setpermN_inv. unfold proj_sumbool. destruct (zle lo ofs). destruct (zlt ofs hi).
   simpl. intros. apply perm_implies with p. apply perm_implies with Freeable. apply perm_cur.
   apply r. tauto. auto with mem. auto.
@@ -2827,15 +2771,15 @@ Proof.
   intros.
   rewrite (store_mem_contents _ _ _ _ _ _ H0).
   rewrite (store_mem_contents _ _ _ _ _ _ STORE).
-  rewrite ! NMap.gsspec.
-  destruct (NMap.elt_eq b0 b1). subst b0.
+  rewrite ! PMap.gsspec.
+  destruct (peq b0 b1). subst b0.
   (* block = b1, block = b2 *)
   assert (b3 = b2) by congruence. subst b3.
   assert (delta0 = delta) by congruence. subst delta0.
   rewrite neq_true.
   apply setN_inj with (access := fun ofs => perm m1 b1 ofs Cur Readable).
   apply encode_val_inject; auto. intros. eapply mi_memval; eauto. eauto with mem.
-  destruct (NMap.elt_eq b3 b2). subst b3.
+  destruct (peq b3 b2). subst b3.
   (* block <> b1, block = b2 *)
   rewrite setN_other. eapply mi_memval; eauto. eauto with mem.
   rewrite encode_val_length. rewrite <- size_chunk_conv. intros.
@@ -2864,7 +2808,7 @@ Proof.
 (* mem_contents *)
   intros.
   rewrite (store_mem_contents _ _ _ _ _ _ H0).
-  setoid_rewrite NMap.gso. eapply mi_memval; eauto with mem.
+  setoid_rewrite PMap.gso. eapply mi_memval; eauto with mem.
   congruence.
 Qed.
 
@@ -2886,7 +2830,7 @@ Proof.
 (* mem_contents *)
   intros.
   rewrite (store_mem_contents _ _ _ _ _ _ H1).
-  rewrite NMap.gsspec. destruct (NMap.elt_eq b2 b). subst b2.
+  rewrite PMap.gsspec. destruct (peq b2 b). subst b2.
   rewrite setN_outside. auto.
   rewrite encode_val_length. rewrite <- size_chunk_conv.
   destruct (zlt (ofs0 + delta) ofs); auto.
@@ -2929,13 +2873,13 @@ Proof.
   assert (perm m1 b0 ofs0 Cur Readable). eapply perm_storebytes_2; eauto.
   rewrite (storebytes_mem_contents _ _ _ _ _ H0).
   rewrite (storebytes_mem_contents _ _ _ _ _ STORE).
-  rewrite ! NMap.gsspec. destruct (NMap.elt_eq b0 b1). subst b0.
+  rewrite ! PMap.gsspec. destruct (peq b0 b1). subst b0.
   (* block = b1, block = b2 *)
   assert (b3 = b2) by congruence. subst b3.
   assert (delta0 = delta) by congruence. subst delta0.
   rewrite neq_true.
   apply setN_inj with (access := fun ofs => perm m1 b1 ofs Cur Readable); auto.
-  destruct (NMap.elt_eq b3 b2). subst b3.
+  destruct (peq b3 b2). subst b3.
   (* block <> b1, block = b2 *)
   rewrite setN_other. auto.
   intros.
@@ -2967,7 +2911,7 @@ Proof.
 (* mem_contents *)
   intros.
   rewrite (storebytes_mem_contents _ _ _ _ _ H0).
-  setoid_rewrite NMap.gso. eapply mi_memval0; eauto. eapply perm_storebytes_2; eauto.
+  setoid_rewrite PMap.gso. eapply mi_memval0; eauto. eapply perm_storebytes_2; eauto.
   congruence.
 Qed.
 
@@ -2989,7 +2933,7 @@ Proof.
 (* mem_contents *)
   intros.
   rewrite (storebytes_mem_contents _ _ _ _ _ H1).
-  rewrite NMap.gsspec. destruct (NMap.elt_eq b2 b). subst b2.
+  rewrite PMap.gsspec. destruct (peq b2 b). subst b2.
   rewrite setN_outside. auto.
   destruct (zlt (ofs0 + delta) ofs); auto.
   destruct (zle (ofs + Z.of_nat (length bytes2)) (ofs0 + delta)). lia.
@@ -3018,8 +2962,8 @@ Proof.
   assert (perm m1 b0 ofs Cur Readable). eapply perm_storebytes_2; eauto.
   rewrite (storebytes_mem_contents _ _ _ _ _ H0).
   rewrite (storebytes_mem_contents _ _ _ _ _ H1).
-  simpl. rewrite ! NMap.gsspec.
-  destruct (NMap.elt_eq b0 b1); destruct (NMap.elt_eq b3 b2); subst; eapply mi_memval0; eauto.
+  simpl. rewrite ! PMap.gsspec.
+  destruct (peq b0 b1); destruct (peq b3 b2); subst; eapply mi_memval0; eauto.
 Qed.
 
 (** Preservation of allocations *)
@@ -3041,7 +2985,7 @@ Proof.
   assert (perm m2 b0 (ofs + delta) Cur Readable).
     eapply mi_perm0; eauto.
   assert (valid_block m2 b0) by eauto with mem.
-  rewrite <- MEM; simpl. setoid_rewrite NMap.gso. eauto with mem.
+  rewrite <- MEM; simpl. setoid_rewrite PMap.gso. eauto with mem.
   rewrite NEXT. eauto with mem.
 Qed.
 
@@ -3064,7 +3008,7 @@ Proof.
   injection H0; intros NEXT MEM. intros.
   rewrite <- MEM; simpl. rewrite NEXT.
   exploit perm_alloc_inv; eauto. intros.
-  rewrite NMap.gsspec. (*unfold eq_block in H4.*) destruct (NMap.elt_eq b0 b1).
+  rewrite PMap.gsspec. (*unfold eq_block in H4.*) destruct (peq b0 b1).
   rewrite ZMap.gi. constructor. apply mi_memval0. auto. eapply perm_alloc_4 in H0. apply H0. auto. auto.
 Qed.
 
@@ -3100,8 +3044,8 @@ Proof.
   injection H0; intros NEXT MEM.
   intros. rewrite <- MEM; simpl. rewrite NEXT.
   exploit perm_alloc_inv; eauto. intros.
-  rewrite NMap.gsspec.
-  destruct (NMap.elt_eq b0 b1). rewrite ZMap.gi. constructor.
+  rewrite PMap.gsspec.
+  destruct (peq b0 b1). rewrite ZMap.gi. constructor.
   apply mi_memval. auto. auto. eapply perm_alloc_4 in H0. eauto. auto. auto.
 Qed.
 
@@ -3261,7 +3205,7 @@ Qed.
 
 Record extends' (m1 m2: mem) : Prop :=
   mk_extends {
-    mext_sup: support m1 = support m2;
+    mext_next: nextblock m1 = nextblock m2;
     mext_inj:  mem_inj inject_id m1 m2;
     mext_perm_inv: forall b ofs k p,
       perm m2 b ofs k p ->
@@ -3334,8 +3278,8 @@ Proof.
   exists m2'; split.
   replace (ofs + 0) with ofs in A by lia. auto.
   constructor; auto.
-  rewrite (support_store _ _ _ _ _ _ H0).
-  rewrite (support_store _ _ _ _ _ _ A).
+  rewrite (nextblock_store _ _ _ _ _ _ H0).
+  rewrite (nextblock_store _ _ _ _ _ _ A).
   auto.
   intros. exploit mext_perm_inv0; intuition eauto using perm_store_1, perm_store_2.
 Qed.
@@ -3348,7 +3292,7 @@ Theorem store_outside_extends:
   extends m1 m2'.
 Proof.
   intros. inversion H. constructor.
-  rewrite (support_store _ _ _ _ _ _ H0). auto.
+  rewrite (nextblock_store _ _ _ _ _ _ H0). auto.
   eapply store_outside_inj; eauto.
   unfold inject_id; intros. inv H2. eapply H1; eauto. lia.
   intros. eauto using perm_store_2.
@@ -3386,8 +3330,8 @@ Proof.
   exists m2'; split.
   replace (ofs + 0) with ofs in A by lia. auto.
   constructor; auto.
-  rewrite (support_storebytes _ _ _ _ _ H0).
-  rewrite (support_storebytes _ _ _ _ _ A).
+  rewrite (nextblock_storebytes _ _ _ _ _ H0).
+  rewrite (nextblock_storebytes _ _ _ _ _ A).
   auto.
   intros. exploit mext_perm_inv0; intuition eauto using perm_storebytes_1, perm_storebytes_2.
 Qed.
@@ -3400,7 +3344,7 @@ Theorem storebytes_outside_extends:
   extends m1 m2'.
 Proof.
   intros. inversion H. constructor.
-  rewrite (support_storebytes _ _ _ _ _ H0). auto.
+  rewrite (nextblock_storebytes _ _ _ _ _ H0). auto.
   eapply storebytes_outside_inj; eauto.
   unfold inject_id; intros. inv H2. eapply H1; eauto. lia.
   intros. eauto using perm_storebytes_2.
@@ -3421,12 +3365,12 @@ Proof.
     rewrite (alloc_result _ _ _ _ _ H0).
     rewrite (alloc_result _ _ _ _ _ ALLOC).
     auto.
-  unfold nextblock. congruence. subst b'.
+    subst b'.
   exists m2'; split; auto.
   constructor.
-  rewrite (support_alloc _ _ _ _ _ H0).
-  rewrite (support_alloc _ _ _ _ _ ALLOC).
-  unfold nextblock. congruence.
+  rewrite (nextblock_alloc _ _ _ _ _ H0).
+  rewrite (nextblock_alloc _ _ _ _ _ ALLOC).
+  congruence.
   eapply alloc_left_mapped_inj with (m1 := m1) (m2 := m2') (b2 := b) (delta := 0); eauto.
   eapply alloc_right_inj; eauto.
   eauto with mem.
@@ -3453,7 +3397,7 @@ Theorem free_left_extends:
   extends m1' m2.
 Proof.
   intros. inv H. constructor.
-  rewrite (support_free _ _ _ _ _ H0). auto.
+  rewrite (nextblock_free _ _ _ _ _ H0). auto.
   eapply free_left_inj; eauto.
   intros. exploit mext_perm_inv0; eauto. intros [A|A].
   eapply perm_free_inv in A; eauto. destruct A as [[A B]|A]; auto.
@@ -3469,7 +3413,7 @@ Theorem free_right_extends:
   extends m1 m2'.
 Proof.
   intros. inv H. constructor.
-  rewrite (support_free _ _ _ _ _ H0). auto.
+  rewrite (nextblock_free _ _ _ _ _ H0). auto.
   eapply free_right_inj; eauto.
   unfold inject_id; intros. inv H. eapply H1; eauto. lia.
   intros. eauto using perm_free_3.
@@ -3491,8 +3435,8 @@ Proof.
     eapply free_range_perm; eauto.
   destruct X as [m2' FREE]. exists m2'; split; auto.
   constructor.
-  rewrite (support_free _ _ _ _ _ H0).
-  rewrite (support_free _ _ _ _ _ FREE). auto.
+  rewrite (nextblock_free _ _ _ _ _ H0).
+  rewrite (nextblock_free _ _ _ _ _ FREE). auto.
   eapply free_right_inj with (m1 := m1'); eauto.
   eapply free_left_inj; eauto.
   unfold inject_id; intros. inv H1.
@@ -3508,7 +3452,7 @@ Theorem valid_block_extends:
   extends m1 m2 ->
   (valid_block m1 b <-> valid_block m2 b).
 Proof.
-  intros. inv H. unfold valid_block. rewrite mext_sup0. tauto.
+  intros. inv H. unfold valid_block. rewrite mext_next0. tauto.
 Qed.
 
 Theorem perm_extends:
@@ -3601,7 +3545,7 @@ Theorem valid_block_inject_1:
   inject f m1 m2 ->
   valid_block m1 b1.
 Proof.
-  intros. inv H. destruct (sup_dec b1 (support m1)). auto.
+  intros. inv H. destruct (plt b1 (nextblock m1)). auto.
   assert (f b1 = None). eapply mi_freeblocks; eauto. congruence.
 Qed.
 
@@ -4425,7 +4369,7 @@ Lemma drop_outside_inject: forall f m1 m2 b lo hi p m2',
 Proof.
   intros. destruct H. constructor; eauto.
   eapply drop_outside_inj; eauto.
-  intros. unfold valid_block in *. erewrite support_drop; eauto.
+  intros. unfold valid_block in *. erewrite nextblock_drop; eauto.
   intros. eapply mi_perm_inv0; eauto using perm_drop_4.
 Qed.
 
@@ -4591,23 +4535,23 @@ Qed.
 
 (** Injecting a memory into itself. *)
 
-Definition flat_inj (s: sup) : meminj :=
-  fun (b: block) => if sup_dec b s then Some(b, 0) else None.
+Definition flat_inj (thr: block) : meminj :=
+  fun (b: block) => if plt b thr then Some(b, 0) else None.
 
-Definition inject_neutral (s: sup) (m: mem) :=
-  mem_inj (flat_inj s) m m.
+Definition inject_neutral (thr: block) (m: mem) :=
+  mem_inj (flat_inj thr) m m.
 
 Remark flat_inj_no_overlap:
-  forall s m, meminj_no_overlap (flat_inj s) m.
+  forall thr m, meminj_no_overlap (flat_inj thr) m.
 Proof.
   unfold flat_inj; intros; red; intros.
-  destruct (sup_dec b1 s); inversion H0; subst.
-  destruct (sup_dec b2 s); inversion H1; subst.
+  destruct (plt b1 thr); inversion H0; subst.
+  destruct (plt b2 thr); inversion H1; subst.
   auto.
 Qed.
 
 Theorem neutral_inject:
-  forall m, inject_neutral (support m) m -> inject (flat_inj (support m)) m m.
+  forall m, inject_neutral (nextblock m) m -> inject (flat_inj (nextblock m)) m m.
 Proof.
   intros. constructor.
 (* meminj *)
@@ -4617,37 +4561,37 @@ Proof.
   apply pred_dec_false. auto.
 (* mappedblocks *)
   unfold flat_inj, valid_block; intros.
-  destruct (sup_dec b (support m)); inversion H0; subst. auto.
+  destruct (plt b (nextblock m)); inversion H0; subst. auto.
 (* no overlap *)
   apply flat_inj_no_overlap.
 (* range *)
   unfold flat_inj; intros.
-  destruct (sup_dec b (support m)); inv H0. generalize (Ptrofs.unsigned_range_2 ofs); lia.
+  destruct (plt b (nextblock m)); inv H0. generalize (Ptrofs.unsigned_range_2 ofs); lia.
 (* perm inv *)
   unfold flat_inj; intros.
-  destruct (sup_dec b1 (support m)); inv H0.
+  destruct (plt b1 (nextblock m)); inv H0.
   rewrite Z.add_0_r in H1; auto.
 Qed.
 
 Theorem empty_inject_neutral:
-  forall s, inject_neutral s empty.
+  forall thr, inject_neutral thr empty.
 Proof.
   intros; red; constructor.
 (* perm *)
-  unfold flat_inj; intros. destruct (sup_dec b1 s); inv H.
+  unfold flat_inj; intros. destruct (plt b1 thr); inv H.
   replace (ofs + 0) with ofs by lia; auto.
 (* align *)
-  unfold flat_inj; intros. destruct (sup_dec b1 s); inv H. apply Z.divide_0_r.
+  unfold flat_inj; intros. destruct (plt b1 thr); inv H. apply Z.divide_0_r.
 (* mem_contents *)
-  intros; simpl. unfold NMap.get. rewrite ! NMap.gi. rewrite ! ZMap.gi. constructor.
+  intros; simpl. rewrite ! PMap.gi. rewrite ! ZMap.gi. constructor.
 Qed.
 
 Theorem alloc_inject_neutral:
-  forall s m lo hi b m',
+  forall thr m lo hi b m',
   alloc m lo hi = (m', b) ->
-  inject_neutral s m ->
-  sup_include (sup_incr (support m)) s ->
-  inject_neutral s m'.
+  inject_neutral thr m ->
+  Plt (nextblock m) thr ->
+  inject_neutral thr m'.
 Proof.
   intros; red.
   eapply alloc_left_mapped_inj with (m1 := m) (b2 := b) (delta := 0).
@@ -4657,17 +4601,17 @@ Proof.
   apply perm_implies with Freeable; auto with mem.
   eapply perm_alloc_2; eauto. lia.
   unfold flat_inj. apply pred_dec_true.
-  apply H1. apply alloc_result in H. subst.
-  apply sup_incr_in1.
+  rewrite (alloc_result _ _ _ _ _ H). auto.
 Qed.
 
+
 Theorem store_inject_neutral:
-  forall chunk m b ofs v m' s,
+  forall chunk m b ofs v m' thr,
   store chunk m b ofs v = Some m' ->
-  inject_neutral s m ->
-  sup_In b s->
-  Val.inject (flat_inj s) v v ->
-  inject_neutral s m'.
+  inject_neutral thr m ->
+  Plt b thr ->
+  Val.inject (flat_inj thr) v v ->
+  inject_neutral thr m'.
 Proof.
   intros; red.
   exploit store_mapped_inj. eauto. eauto. apply flat_inj_no_overlap.
@@ -4677,11 +4621,11 @@ Proof.
 Qed.
 
 Theorem drop_inject_neutral:
-  forall m b lo hi p m' s,
+  forall m b lo hi p m' thr,
   drop_perm m b lo hi p = Some m' ->
-  inject_neutral s m ->
-  sup_In b s ->
-  inject_neutral s m'.
+  inject_neutral thr m ->
+  Plt b thr ->
+  inject_neutral thr m'.
 Proof.
   unfold inject_neutral; intros.
   exploit drop_mapped_inj; eauto. apply flat_inj_no_overlap.
@@ -4696,8 +4640,8 @@ Section UNCHANGED_ON.
 Variable P: block -> Z -> Prop.
 
 Record unchanged_on (m_before m_after: mem) : Prop := mk_unchanged_on {
-  unchanged_on_support:
-    sup_include (support m_before) (support m_after);
+  unchanged_on_nextblock:
+    Ple (nextblock m_before) (nextblock m_after);
   unchanged_on_perm:
     forall b ofs k p,
     P b ofs -> valid_block m_before b ->
@@ -4705,21 +4649,21 @@ Record unchanged_on (m_before m_after: mem) : Prop := mk_unchanged_on {
   unchanged_on_contents:
     forall b ofs,
     P b ofs -> perm m_before b ofs Cur Readable ->
-    ZMap.get ofs (NMap.get _ b m_after.(mem_contents)) =
-    ZMap.get ofs (NMap.get _ b m_before.(mem_contents))
+    ZMap.get ofs (PMap.get b m_after.(mem_contents)) =
+    ZMap.get ofs (PMap.get b m_before.(mem_contents))
 }.
 
 Lemma unchanged_on_refl:
   forall m, unchanged_on m m.
 Proof.
-  intros; constructor. apply sup_include_refl. tauto. tauto.
+  intros; constructor. apply Ple_refl. tauto. tauto.
 Qed.
 
 Lemma valid_block_unchanged_on:
   forall m m' b,
   unchanged_on m m' -> valid_block m b -> valid_block m' b.
 Proof.
-  unfold valid_block; intros. apply unchanged_on_support in H. auto.
+  unfold valid_block; intros. apply unchanged_on_nextblock in H. extlia.
 Qed.
 
 Lemma perm_unchanged_on:
@@ -4742,7 +4686,7 @@ Lemma unchanged_on_trans:
   forall m1 m2 m3, unchanged_on m1 m2 -> unchanged_on m2 m3 -> unchanged_on m1 m3.
 Proof.
   intros; constructor.
-- apply sup_include_trans with (support m2); apply unchanged_on_support; auto.
+- apply Ple_trans with (nextblock m2); apply unchanged_on_nextblock; auto.
 - intros. transitivity (perm m2 b ofs k p); apply unchanged_on_perm; auto.
   eapply valid_block_unchanged_on; eauto.
 - intros. transitivity (ZMap.get ofs (mem_contents m2)#b); apply unchanged_on_contents; auto.
@@ -4816,10 +4760,10 @@ Lemma store_unchanged_on:
   unchanged_on m m'.
 Proof.
   intros; constructor; intros.
-- rewrite (support_store _ _ _ _ _ _ H). apply sup_include_refl.
+- rewrite (nextblock_store _ _ _ _ _ _ H). apply Ple_refl.
 - split; intros; eauto with mem.
-- erewrite store_mem_contents; eauto. rewrite NMap.gsspec.
-  destruct (NMap.elt_eq b0 b); auto. subst b0. apply setN_outside.
+- erewrite store_mem_contents; eauto. rewrite PMap.gsspec.
+  destruct (peq b0 b); auto. subst b0. apply setN_outside.
   rewrite encode_val_length. rewrite <- size_chunk_conv.
   destruct (zlt ofs0 ofs); auto.
   destruct (zlt ofs0 (ofs + size_chunk chunk)); auto.
@@ -4833,10 +4777,10 @@ Lemma storebytes_unchanged_on:
   unchanged_on m m'.
 Proof.
   intros; constructor; intros.
-- rewrite (support_storebytes _ _ _ _ _ H). apply sup_include_refl.
+- rewrite (nextblock_storebytes _ _ _ _ _ H). apply Ple_refl.
 - split; intros. eapply perm_storebytes_1; eauto. eapply perm_storebytes_2; eauto.
-- erewrite storebytes_mem_contents; eauto. rewrite NMap.gsspec.
-  destruct (NMap.elt_eq b0 b); auto. subst b0. apply setN_outside.
+- erewrite storebytes_mem_contents; eauto. rewrite PMap.gsspec.
+  destruct (peq b0 b); auto. subst b0. apply setN_outside.
   destruct (zlt ofs0 ofs); auto.
   destruct (zlt ofs0 (ofs + Z.of_nat (length bytes))); auto.
   elim (H0 ofs0). lia. auto.
@@ -4848,13 +4792,13 @@ Lemma alloc_unchanged_on:
   unchanged_on m m'.
 Proof.
   intros; constructor; intros.
-- rewrite (support_alloc _ _ _ _ _ H). intro. intro. apply sup_incr_in2. auto.
+- rewrite (nextblock_alloc _ _ _ _ _ H). apply Ple_succ.
 - split; intros.
   eapply perm_alloc_1; eauto.
   eapply perm_alloc_4; eauto.
   eapply valid_not_valid_diff; eauto with mem.
 - injection H; intros A B. rewrite <- B; simpl.
-  setoid_rewrite NMap.gso; auto. rewrite A.  eapply valid_not_valid_diff; eauto with mem.
+  setoid_rewrite PMap.gso; auto. rewrite A.  eapply valid_not_valid_diff; eauto with mem.
 Qed.
 
 Lemma free_unchanged_on:
@@ -4864,7 +4808,7 @@ Lemma free_unchanged_on:
   unchanged_on m m'.
 Proof.
   intros; constructor; intros.
-- rewrite (support_free _ _ _ _ _ H). apply sup_include_refl.
+- rewrite (nextblock_free _ _ _ _ _ H). apply Ple_refl.
 - split; intros.
   eapply perm_free_1; eauto.
   destruct (eq_block b0 b); auto. destruct (zlt ofs lo); auto. destruct (zle hi ofs); auto.
@@ -4881,7 +4825,7 @@ Lemma free_unchanged_on':
   unchanged_on m' m.
 Proof.
   intros; constructor; intros.
-- rewrite (support_free _ _ _ _ _ H). apply sup_include_refl.
+- rewrite (nextblock_free _ _ _ _ _ H). apply Ple_refl.
 - split; intros.
   eapply perm_free_3; eauto.
   eapply perm_free_1; eauto.
@@ -4898,7 +4842,7 @@ Lemma drop_perm_unchanged_on:
   unchanged_on m m'.
 Proof.
   intros; constructor; intros.
-- rewrite (support_drop _ _ _ _ _ _ H). apply sup_include_refl.
+- rewrite (nextblock_drop _ _ _ _ _ _ H). apply Ple_refl.
 - split; intros. eapply perm_drop_3; eauto.
   destruct (eq_block b0 b); auto.
   subst b0.
@@ -4942,10 +4886,10 @@ Proof.
     eapply perm_valid_block. eapply RANGE1. instantiate (1:= ofs). lia.
   }
   destruct X as [n2 STORE2].
-  apply support_store in STORE1 as SUP1. apply support_store in STORE2 as SUP2.
+  apply nextblock_store in STORE1 as NEXT1. apply nextblock_store in STORE2 as NEXT2.
   exists n2. split. auto. inversion UNC1.
   constructor.
-  - rewrite SUP1, SUP2. eauto.
+  - rewrite NEXT1, NEXT2. eauto.
   - intros. split; intros.
     eapply perm_store_1; eauto. eapply unchanged_on_perm0; eauto.
     unfold valid_block in *. congruence. eapply perm_store_2; eauto.
@@ -4961,9 +4905,9 @@ Proof.
     inv STORE1. inv STORE2. cbn in *.
     unfold perm in H0. simpl in H0.
     destruct (eq_block b b0). subst.
-    rewrite !NMap.gss.
+    rewrite !PMap.gss.
     eapply setN_remain_same; eauto.
-    rewrite !NMap.gso; eauto.
+    rewrite !PMap.gso; eauto.
 Qed.
 
 Lemma free_mapped_unchanged_on : forall m1 b lo hi m2 n1,
@@ -4984,22 +4928,22 @@ Proof.
     eapply perm_valid_block. eapply RANGE1. instantiate (1:= ofs). lia.
   }
   destruct X as [n2 FREE2].
-  apply support_free in FREE1 as SUP1. apply support_free in FREE2 as SUP2.
+  apply nextblock_free in FREE1 as NEXT1. apply nextblock_free in FREE2 as NEXT2.
   exists n2. split. auto. inversion UNC1.
   constructor.
-  - rewrite SUP1, SUP2. eauto.
+  - rewrite NEXT1, NEXT2. eauto.
   - intros.
     apply free_result in FREE1. apply free_result in FREE2.
     subst. unfold perm. cbn.
     destruct (eq_block b0 b); auto.
     + (*same block*) subst.
-       rewrite !NMap.gss.
+       rewrite !PMap.gss.
       destruct (zle lo ofs); destruct (zle hi ofs); auto.
       -- rewrite !setpermN_outside; try lia. eauto.
       -- rewrite !setpermN_inside; try lia. reflexivity.
       -- rewrite !setpermN_outside; try lia. eauto.
       -- rewrite !setpermN_outside; try lia. eauto.
-    + rewrite !NMap.gso; eauto.
+    + rewrite !PMap.gso; eauto.
   - intros. apply free_result in FREE1 as RES1. apply free_result in FREE2.
     subst. simpl. eapply unchanged_on_contents0; eauto.
     eapply Mem.perm_free_3; eauto.
@@ -5035,7 +4979,7 @@ Definition ro_unchanged_memval m m' : Prop :=
       perm m' b ofs Cur Readable ->
       ~ perm m b ofs Max Writable ->
       perm m b ofs Cur Readable /\
-        ZMap.get ofs (NMap.get _ b (mem_contents m)) = ZMap.get ofs (NMap.get _ b (mem_contents m')).
+        ZMap.get ofs (PMap.get b (mem_contents m)) = ZMap.get ofs (PMap.get b (mem_contents m')).
 
 Lemma ro_unchanged_memval_bytes: forall m m',
     ro_unchanged m m' <-> ro_unchanged_memval m m'.
@@ -5043,7 +4987,7 @@ Proof.
   intros. split.
   - intros. red in H. red. intros.
     exploit H. eauto. instantiate (2:= 1).
-    instantiate (2:= ofs). instantiate (1:= ZMap.get ofs (NMap.get _ b (mem_contents m')) :: nil).
+    instantiate (2:= ofs). instantiate (1:= ZMap.get ofs (PMap.get b (mem_contents m')) :: nil).
     unfold loadbytes. destruct range_perm_dec.
     simpl. reflexivity. exfalso. apply n. red.
     intros. destruct (zeq ofs0 ofs). subst. eauto. extlia.
@@ -5113,33 +5057,38 @@ Proof.
     + left. auto.
 Qed.
 
+Lemma storebytes_nil_loadbytes :forall m m' b ofs b1 ofs1 bytes n,
+    storebytes m b ofs nil = Some m' ->
+    loadbytes m' b1 ofs1 n = Some bytes ->
+    loadbytes m b1 ofs1 n = Some bytes.
+Admitted.
+
 Lemma ro_unchanged_storebytes :forall m m' b ofs bytes,
     storebytes m b ofs bytes = Some m' -> ro_unchanged m m'.
 Proof.
   intros. red. intros.
   destruct (Z_le_gt_dec n 0).
+  -
     rewrite Mem.loadbytes_empty in H1; eauto. inv H1.
     rewrite Mem.loadbytes_empty. eauto. auto.
-    destruct (Z_le_gt_dec (Z.of_nat (Datatypes.length bytes)) 0).
+  - destruct (Z_le_gt_dec (Z.of_nat (Datatypes.length bytes)) 0).
     destruct bytes. simpl in l. inv H.
-    assert (m = m'). {
-      eapply Mem.storebytes_empty; eauto.
-    }
-    subst. eauto. cbn in l. extlia.
-    erewrite <- Mem.loadbytes_storebytes_other; eauto. lia.
-    apply Mem.storebytes_range_perm in H. red in H.
-    destruct (eq_block b0 b). subst. right.
-    destruct (Z_le_gt_dec (ofs0+n) ofs).
-    left. auto.
-    destruct (Z_le_gt_dec (ofs + Z.of_nat (Datatypes.length bytes)) ofs0).
-    right. auto.
-    exfalso.
-    destruct (Z_le_gt_dec ofs ofs0).
-    exploit H. instantiate (1:= ofs0). lia. intro PERM.
-    exploit H2. instantiate (1:= ofs0). lia.  eauto with mem. auto.
-    exploit H. instantiate (1:= ofs). lia. intro PERM.
-    exploit H2. instantiate (1:= ofs). lia. eauto with mem. auto.
-    left. auto.
+    + eapply storebytes_nil_loadbytes; eauto.
+    + cbn in l. extlia.
+    + erewrite <- Mem.loadbytes_storebytes_other; eauto. lia.
+      apply Mem.storebytes_range_perm in H. red in H.
+      destruct (eq_block b0 b). subst. right.
+      destruct (Z_le_gt_dec (ofs0+n) ofs).
+      left. auto.
+      destruct (Z_le_gt_dec (ofs + Z.of_nat (Datatypes.length bytes)) ofs0).
+      right. auto.
+      exfalso.
+      destruct (Z_le_gt_dec ofs ofs0).
+      exploit H. instantiate (1:= ofs0). lia. intro PERM.
+      exploit H2. instantiate (1:= ofs0). lia.  eauto with mem. auto.
+      exploit H. instantiate (1:= ofs). lia. intro PERM.
+      exploit H2. instantiate (1:= ofs). lia. eauto with mem. auto.
+      left. auto.
 Qed.
 
 Definition max_perm_decrease (m m': mem) :=
@@ -5150,12 +5099,13 @@ Definition max_perm_decrease (m m': mem) :=
 
 Lemma ro_unchanged_trans: forall m1 m2 m3,
     ro_unchanged m1 m2 -> ro_unchanged m2 m3 ->
-    sup_include (support m1) (support m2) ->
+    Ple (nextblock m1) (nextblock m2) ->
     max_perm_decrease m1 m2 ->
     ro_unchanged m1 m3.
 Proof.
   intros. red. intros. eapply H; eauto.
-  eapply H0; eauto. eapply H1; eauto.
+  eapply H0; eauto.
+  eapply Plt_Ple_trans; eauto.
   intros. intro. eapply H5; eauto.
 Qed.
 
@@ -5224,8 +5174,8 @@ Qed.
 (** [mix m' b lo hi m] copies the region indicated by [b], [lo], [hi]
   from [m] into [m']. *)
 
-Definition pmap_update {A} b (f : A -> A) (t : NMap.t A) : NMap.t A :=
-  NMap.set A b (f (NMap.get A b t)) t.
+Definition pmap_update {A} b (f : A -> A) (t : PMap.t A) : PMap.t A :=
+  PMap.set b (f (PMap.get b t)) t.
 
 Fixpoint update_elements' (lo:Z) (l:nat) (pm: ZMap.t (perm_kind -> option permission)) :=
   match l with
@@ -5314,62 +5264,60 @@ Proof.
 Qed.
 
 Definition mixable m' b m :=
-  sup_include (support m) (support m') /\
+  Pos.le (nextblock m) (nextblock m') /\
   Mem.valid_block m b.
 
 Lemma mixable_dec m' b m :
   {mixable m' b m} + {~ mixable m' b m}.
 Proof.
   unfold mixable, valid_block.
-  destruct (sup_include_dec (support m) (support m')).
-  - destruct (sup_dec b (support m)).
-    + left. auto.
-    + right. intro. apply n. apply H.
-  - right. intro. apply n. apply H.
+  destruct (Pos.leb (nextblock m) (nextblock m')) eqn:Hnb.
+  - apply Pos.leb_le in Hnb.
+    destruct (Pos.ltb b (nextblock m)) eqn:Hb.
+    + apply Pos.ltb_lt in Hb. left. auto.
+    + apply Pos.ltb_nlt in Hb. right. tauto.
+  - apply Pos.leb_nle in Hnb. right. tauto.
 Qed.
 
 Program Definition mix m' b lo hi m : option mem :=
   if mixable_dec m' b m then
     Some {|
       mem_contents :=
-        let bytes := Mem.getN (Z.to_nat (hi - lo)) lo (NMap.get _ b (Mem.mem_contents m)) in
+        let bytes := Mem.getN (Z.to_nat (hi - lo)) lo (PMap.get b (Mem.mem_contents m)) in
         pmap_update b (Mem.setN bytes lo) (Mem.mem_contents m');
       mem_access :=
-        let perms := NMap.get _ b (Mem.mem_access m) in
+        let perms := PMap.get b (Mem.mem_access m) in
         pmap_update b (mix_perms lo hi perms) (Mem.mem_access m');
-      support :=
-        Mem.support m';
+      nextblock :=
+        Mem.nextblock m';
     |}
   else
     None.
 Next Obligation.
   unfold pmap_update. destruct (eq_block b0 b); subst.
-  - rewrite NMap.gsspec.
+  - rewrite PMap.gsspec.
     rewrite pred_dec_true.
     repeat rewrite mix_perms_result.
     destruct (_ && _); apply Mem.access_max. auto.
-  - rewrite NMap.gsspec. rewrite pred_dec_false.
+  - rewrite PMap.gsspec. rewrite pred_dec_false.
     apply Mem.access_max. auto.
 Qed.
 Next Obligation.
   unfold pmap_update. destruct H as [? ?]. unfold valid_block in *.
-  rewrite NMap.gsspec. rewrite pred_dec_false.
+  rewrite PMap.gso by extlia.
   apply Mem.nextblock_noaccess; auto.
-  intro. subst. apply H0. apply H,H1.
 Qed.
 Next Obligation.
   unfold pmap_update. destruct (eq_block b0 b); subst.
-  - rewrite NMap.gsspec. rewrite pred_dec_true; auto.
-    rewrite Mem.setN_default. apply Mem.contents_default.
-  - rewrite NMap.gsspec. rewrite pred_dec_false; auto.
-    apply Mem.contents_default.
+  - rewrite PMap.gss. rewrite Mem.setN_default. apply Mem.contents_default.
+  - rewrite PMap.gso by auto. apply Mem.contents_default.
 Qed.
 Next Obligation.
   unfold pmap_update. destruct (eq_block b0 b); subst.
-  - rewrite NMap.gsspec. rewrite pred_dec_true; auto.
+  - rewrite PMap.gsspec. rewrite pred_dec_true; auto.
     unfold mix_perms.
     rewrite Mem.setN'_default. apply Mem.access_default.
-  - rewrite NMap.gsspec. rewrite pred_dec_false; auto.
+  - rewrite PMap.gsspec. rewrite pred_dec_false; auto.
     apply Mem.access_default.
 Qed.
 
@@ -5386,7 +5334,7 @@ Qed.
 
 Theorem valid_block_mix:
   forall m' b lo hi m,
-  sup_include (support m) (support m') ->
+  Ple (nextblock m) (nextblock m') ->
   valid_block m b ->
   exists m'', mix m' b lo hi m = Some m''.
 Proof.
@@ -5424,7 +5372,7 @@ Qed.
 Theorem support_mix:
   forall m' b lo hi m m'',
   mix m' b lo hi m = Some m'' ->
-  support m'' = support m'.
+  nextblock m'' = nextblock m'.
 Proof.
   unfold mix. intros. destruct mixable_dec; inv H. reflexivity.
 Qed.
@@ -5436,16 +5384,16 @@ Theorem mix_unchanged:
 Proof.
   intros. unfold mix in H. destruct mixable_dec as [[SUP VALID] | ]; inv H.
   constructor; cbn.
-  - apply sup_include_refl.
+  - apply Ple_refl.
   - unfold perm; cbn. intros b1 ofs1 k p H ?.
     unfold pmap_update.
-    destruct (eq_block b1 b); subst; rewrite ?NMap.gss, ?NMap.gso; auto using iff_refl.
+    destruct (eq_block b1 b); subst; rewrite ?PMap.gss, ?PMap.gso; auto using iff_refl.
     rewrite mix_perms_result.
     destruct zle, zlt; cbn; auto using iff_refl.
     elim H; auto.
   - intros b1 ofs1 H Hp.
     unfold pmap_update.
-    destruct (eq_block b1 b); subst; rewrite ?NMap.gss, ?NMap.gso; auto.
+    destruct (eq_block b1 b); subst; rewrite ?PMap.gss, ?PMap.gso; auto.
     rewrite setN_outside; auto.
     destruct (zlt ofs1 lo); auto. right.
     destruct (zlt ofs1 hi); try (elim H; split; auto; extlia).
@@ -5494,11 +5442,11 @@ Proof.
   constructor; cbn.
   - auto.
   - intros _ ofs k p [[ ] Hofs] Hb. unfold perm; cbn.
-    unfold pmap_update. rewrite NMap.gss.
+    unfold pmap_update. rewrite PMap.gss.
     rewrite mix_perms_result.
     destruct zle, zlt; try extlia; cbn. reflexivity.
   - intros _ ofs [[ ] Hofs] Hp.
-    unfold pmap_update. rewrite NMap.gss.
+    unfold pmap_update. rewrite PMap.gss.
     rewrite get_setN_getN; auto.
 Qed.
 
@@ -5674,21 +5622,29 @@ Proof.
       eapply mi_perm_inv; eauto.
 Qed.
 
-(** Memory support extension *)
+(** Memory nextblock extension *)
 
-Program Definition supext (s:sup) (m:mem) : mem :=
-  if (sup_include_dec (Mem.support m) s) then
+Lemma Ple_dec : forall b1 b2, {Ple b1 b2} + {~ Ple b1 b2}.
+Proof.
+  intros. destruct (Pos.leb b1 b2) eqn:H.
+  left. apply Pos.leb_le. eauto.
+  right. apply Pos.leb_nle. eauto.
+Qed.
+
+Program Definition supext (s:block) (m:mem) : mem :=
+  if (Ple_dec (Mem.nextblock m) s) then
     {|
       mem_contents := (mem_contents m);
       mem_access := (mem_access m);
-      support := s
+      nextblock := s
     |} else
     m.
 Next Obligation.
    apply access_max; eauto.
 Qed.
 Next Obligation.
-   apply nextblock_noaccess; eauto.
+  apply nextblock_noaccess. intro. apply H0.
+  eapply Plt_Ple_trans; eauto.
 Qed.
 Next Obligation.
    apply contents_default; eauto.
@@ -6121,7 +6077,7 @@ Proof.
 Qed.
 
 Definition inject_dom_in (f:meminj) s : Prop :=
-  forall b b' o, f b = Some (b',o) -> sup_In b s.
+  forall b b' o, f b = Some (b',o) -> Plt b s.
 
 (**  proof of loc_in_reach_dec which is contained by 
      properties about loc_in_reach_find presented later *)
@@ -6188,33 +6144,33 @@ Qed.
 Section STEP23.
   
 Variable m1 m2 m3 m1' : mem.
-Variable s2' : sup.  
+Variable s2' : block.  
 Variable j12 j23 j12' j23': meminj.
 
 Hypothesis INJ1: inject j12 m1 m2.
 Hypothesis INJ2: inject j23 m2 m3.
-Hypothesis SUPINCR2 : sup_include (support m2) s2'.
+Hypothesis SUPINCR2 : Ple (nextblock m2) s2'.
 
 (** The construction step (2) in appendix *)
 
  Program Definition map_block (b1:block) (m:mem) :=
   match j12' b1 with
   |Some (b2,delta) =>
-     if (sup_dec b1 (Mem.support m1)) then m else
-       if (sup_dec b2 (Mem.support m)) then (* well-typeness constrain *)
+     if (plt b1 (Mem.nextblock m1)) then m else
+       if (plt b2 (Mem.nextblock m)) then (* well-typeness constrain *)
      {|
        mem_contents :=
            pmap_update b2 (update_mem_content ((mem_access m1')#b1) j12' delta (mem_contents m1')#b1)
                        (mem_contents m);
        mem_access :=
            pmap_update b2 (update_mem_access delta (mem_access m1')#b1) (mem_access m);
-       support := (Mem.support m);
+       nextblock := (Mem.nextblock m);
      |} else m
   |None => m
   end.
 Next Obligation.
     unfold pmap_update. destruct (eq_block b b2); subst.
-  - rewrite NMap.gsspec. rewrite pred_dec_true; auto.
+  - rewrite PMap.gsspec. rewrite pred_dec_true; auto.
     generalize (update_mem_access_result delta ).
     intros. erewrite H1; eauto.
     erewrite update_mem_access_result; eauto.
@@ -6222,31 +6178,43 @@ Next Obligation.
     apply Mem.access_max; eauto.
     apply Mem.access_default.
     apply Mem.access_default.
-  - rewrite NMap.gsspec. rewrite pred_dec_false; auto.
+  - rewrite PMap.gsspec. rewrite pred_dec_false; auto.
     apply Mem.access_max; auto.
 Qed.
 Next Obligation.
   unfold pmap_update. destruct (eq_block b b2); subst.
   - congruence.
-  - rewrite NMap.gsspec. rewrite pred_dec_false; auto.
+  - rewrite PMap.gsspec. rewrite pred_dec_false; auto.
     apply Mem.nextblock_noaccess. auto.
 Qed.
 Next Obligation.
     unfold pmap_update. destruct (eq_block b b2); subst.
-  - rewrite NMap.gsspec. rewrite pred_dec_true; auto. unfold update_mem_content.
+  - rewrite PMap.gsspec. rewrite pred_dec_true; auto. unfold update_mem_content.
     rewrite setN'_default. apply Mem.contents_default.
-  - rewrite NMap.gsspec. rewrite pred_dec_false; auto.
+  - rewrite PMap.gsspec. rewrite pred_dec_false; auto.
     apply Mem.contents_default.
 Qed.
 Next Obligation.
     unfold pmap_update. destruct (eq_block b b2); subst.
-  - rewrite NMap.gsspec. rewrite pred_dec_true; auto. unfold update_mem_access.
+  - rewrite PMap.gsspec. rewrite pred_dec_true; auto. unfold update_mem_access.
     rewrite setN'_default. apply Mem.access_default.
-  - rewrite NMap.gsspec. rewrite pred_dec_false; auto.
+  - rewrite PMap.gsspec. rewrite pred_dec_false; auto.
     apply Mem.access_default.
 Qed.
 
-Fixpoint map_sup (s:sup) (m:mem) :=
+Fixpoint map_nextblock (s: block) (m:mem) :=
+  match s with
+  |xH => m
+  |xO s' => map_block s' (map_nextblock s' m)
+  |xI s' => map_block s' (map_block (xO s') (map_nextblock s' m))
+  end.
+
+
+Parameter nb_list : block -> list block.
+Axiom nb_list_correct : forall s b,
+    Plt b s <-> In b (nb_list s).
+
+Fixpoint map_sup (s: list block) (m:mem) :=
   match s with
   |nil => m
   |hd:: tl => map_block hd (map_sup tl m)
@@ -6254,34 +6222,34 @@ Fixpoint map_sup (s:sup) (m:mem) :=
 
 (** step2, with the extension of support s2' which is constructed in step (1) *)
 Definition step2 := 
-  map_sup (support m1') (supext s2' m2).
+  map_sup (nb_list (nextblock m1')) (supext s2' m2).
 
 (** properties of step2 *)
 
 Lemma map_block_support : forall b m,
-  support (map_block b m) = support m.
+  nextblock (map_block b m) = nextblock m.
 Proof.
   intros. unfold map_block.
   destruct (j12' b); auto.
   destruct p.
-  destruct (sup_dec); auto.
-  destruct (sup_dec); auto.
+  destruct (plt); auto.
+  destruct (plt); auto.
 Qed.
 
 Lemma map_sup_support : forall s m,
-    support (map_sup s m) = support m.
+    nextblock (map_sup s m) = nextblock m.
 Proof.
   induction s; intros; simpl; eauto.
   rewrite map_block_support. eauto.
 Qed.
 
 Lemma step2_support :
-  support step2 = s2'.
+  nextblock step2 = s2'.
 Proof.
   unfold step2. rewrite map_sup_support.
   unfold supext.
-  destruct sup_include_dec; eauto.
-  congruence.
+  destruct Ple_dec; eauto.
+  extlia.
 Qed.
 
 (** construction step3 *)
@@ -6292,10 +6260,10 @@ Section REVERSE.
   Variable o2: Z.
   (* Hypothesis PERM2 : perm m2 b2 o2 Max Nonempty. *)
 
-  Lemma DOMIN: inject_dom_in j12 (Mem.support m1).
+  Lemma DOMIN: inject_dom_in j12 (Mem.nextblock m1).
   Proof.
     red. intros. inv INJ1.
-    destruct (sup_dec b (Mem.support m1)).
+    destruct (plt b (Mem.nextblock m1)).
     auto. exploit mi_freeblocks0; eauto.
     intro. congruence.
   Qed.
@@ -6310,7 +6278,7 @@ Section REVERSE.
     match j12 b1 with
     |Some (b2',delta) =>
        if eq_block b2 b2' then
-         let pmap1 := (mem_access m1 b1) in
+         let pmap1 := ((mem_access m1) # b1) in
          let elements := perm_elements_any (ZMap.elements pmap1) in
          match find (check_position (o2 - delta)) elements with
          |Some (o1,_) => Some (b1,o2 - delta)
@@ -6321,7 +6289,7 @@ Section REVERSE.
     end.
 
   (* find (b_1,o_1) in all blocks in s *)
-  Fixpoint loc_in_reach_find' (b2: block) (o2: Z) (s : sup): option (block * Z) :=
+  Fixpoint loc_in_reach_find' (b2: block) (o2: Z) (s : list block): option (block * Z) :=
     match s with
     | nil => None
     | hd :: tl =>
@@ -6333,7 +6301,7 @@ Section REVERSE.
 
   (*specific find function, find (b_1,o_1) in sup(m_1)*)
   Definition loc_in_reach_find (b2: block) (o2: Z) :=
-    loc_in_reach_find' b2 o2 (Mem.support m1).
+    loc_in_reach_find' b2 o2 (nb_list (Mem.nextblock m1)).
 
   Lemma block_find_valid: forall b b2 o2 b1 o1,
       block_find b b2 o2 = Some (b1, o1) ->
@@ -6352,7 +6320,6 @@ Section REVERSE.
     apply in_perm_any_1 in H.
     destruct H as [PERM IN].
     apply ZMap.elements_complete in IN.
-    unfold NMap.get.
     rewrite IN. destruct (m Max); eauto.
     constructor.
   Qed.
@@ -6386,22 +6353,21 @@ Section REVERSE.
     rewrite pred_dec_true in H; eauto.
     destruct find eqn:FIND; try congruence.
     destruct p. inv H.
-
-    assert (forall z, In z (perm_elements_any (ZMap.elements (mem_access m1 b)))
+    assert (forall z, In z (perm_elements_any (ZMap.elements ((mem_access m1)# b)))
                  -> check_position (o0 - d) z = false).
     apply find_none. eauto.
     unfold perm. unfold perm_order'.
     destruct (((mem_access m1) # b) ## (o0 - d) Max) eqn:PERM.
     exploit H0. eapply in_perm_any; eauto.
     eapply elements_correct'. setoid_rewrite access_default.
-    unfold NMap.get in PERM. intro. rewrite H1 in PERM. congruence.
+    intro. rewrite H1 in PERM. congruence.
     unfold check_position. simpl.
     rewrite pred_dec_true; eauto. intro. congruence. eauto.
   Qed.
   
   Lemma loc_in_reach_find'_none_rec : forall s b2 o2,
       loc_in_reach_find' b2 o2 s = None ->
-      forall b1 d1, j12 b1 = Some (b2,d1) -> sup_In b1 s -> ~ perm m1 b1 (o2 - d1) Max Nonempty.
+      forall b1 d1, j12 b1 = Some (b2,d1) -> In b1 s -> ~ perm m1 b1 (o2 - d1) Max Nonempty.
   Proof.
     induction s; intros.
     - inv H1.
@@ -6415,7 +6381,8 @@ Qed.
   Proof.
     intros. unfold loc_in_reach_find in H.
     red. intros. eapply loc_in_reach_find'_none_rec; eauto.
-    inv INJ1. destruct (sup_dec b0 (support m1)). auto.
+    apply nb_list_correct.
+    inv INJ1. destruct (plt b0 (nextblock m1)). auto.
     exploit mi_freeblocks0; eauto.
     intro. congruence.
   Qed.
@@ -6738,7 +6705,7 @@ Proof.
 Qed.
 
 Lemma loc_in_reach_notin2:
-  forall b o, ~ sup_In b (support m2) -> loc_in_reach_find b o = None.
+  forall b o, ~ Plt b (nextblock m2) -> loc_in_reach_find b o = None.
 Proof.
   intros. destruct (loc_in_reach_find b o) as [[b1 o1]|] eqn:FIND; eauto.
   exfalso. apply loc_in_reach_find_valid in FIND. destruct FIND as [A B].
@@ -6749,7 +6716,7 @@ Qed.
 
  Program Definition copy_block b2 m : mem :=
    if j23 b2 then
-      if (sup_dec b2 (Mem.support m)) then
+      if (plt b2 (Mem.nextblock m)) then
       {|
         mem_contents := pmap_update b2
                           (copy_content_block b2)
@@ -6757,13 +6724,13 @@ Qed.
         mem_access := pmap_update b2
                         (copy_access_block b2)
                         (mem_access m);
-        support := (Mem.support m);
+        nextblock := (Mem.nextblock m);
       |}
         else m
    else m.
  Next Obligation.
-   unfold pmap_update. rewrite NMap.gsspec.
-   destruct NMap.elt_eq.
+   unfold pmap_update. rewrite PMap.gsspec.
+   destruct peq.
    - repeat rewrite copy_access_block_result.
      destruct loc_in_reach_find.
      + destruct p. apply access_max.
@@ -6771,27 +6738,27 @@ Qed.
    - apply access_max.
  Qed.
  Next Obligation.
-   unfold pmap_update. rewrite NMap.gsspec.
-   destruct NMap.elt_eq.
+   unfold pmap_update. rewrite PMap.gsspec.
+   destruct peq.
    - subst. congruence.
    - apply nextblock_noaccess; eauto.
  Qed.
  Next Obligation.
-   unfold pmap_update. rewrite NMap.gsspec.
-   destruct NMap.elt_eq.
+   unfold pmap_update. rewrite PMap.gsspec.
+   destruct peq.
    - subst. unfold copy_content_block. rewrite setN'_default.
      apply contents_default.
    - apply contents_default.
  Qed.
  Next Obligation.
-   unfold pmap_update. rewrite NMap.gsspec.
+   unfold pmap_update. rewrite PMap.gsspec.
    destruct eq_block; try apply access_default.
    unfold copy_access_block. rewrite setN'_default.
    apply access_default.
  Qed.
 
 
- Fixpoint copy_sup (s:sup) m : mem :=
+ Fixpoint copy_sup (s:list block) m : mem :=
    match s with
    | nil => m
    | hd :: tl => copy_block hd (copy_sup tl m)
@@ -6800,16 +6767,16 @@ Qed.
  (** lemmas about step3 *)
  Lemma copy_block_support : forall b m m',
      copy_block b m = m' ->
-     support m' = support m.
+     nextblock m' = nextblock m.
  Proof.
    intros. subst. unfold copy_block.
    destruct (j23 b); auto.
-   destruct (sup_dec); auto.
+   destruct (plt); auto.
  Qed.
 
  Lemma copy_sup_support : forall s m m',
      copy_sup s m = m' ->
-     support m' = support m.
+     nextblock m' = nextblock m.
  Proof.
    induction s; intros; subst; simpl; eauto.
    erewrite copy_block_support. 2: eauto.
@@ -6821,22 +6788,9 @@ End STEP23.
 End Mem.
 
 Notation mem := Mem.mem.
-Notation sup := Mem.sup.
-Notation sup_In := Mem.sup_In.
-Notation sup_incr := Mem.sup_incr.
-Notation sup_empty := Mem.sup_empty.
-Notation fresh_block := Mem.fresh_block.
-Notation freshness := Mem.freshness.
 Global Opaque Mem.alloc Mem.free Mem.store Mem.load Mem.storebytes Mem.loadbytes.
 
 
-Global Hint Resolve
-  Mem.sup_incr_in1
-  Mem.sup_incr_in2
-  Mem.sup_include_refl
-  Mem.sup_include_trans
-  Mem.sup_include_incr
-  : core.
 Global Hint Resolve
   Mem.valid_not_valid_diff
   Mem.perm_implies
